*****************
funciones inversa
*****************

dadas :math: `f( x ) = 3x + 2` y :math: `g( x ) = \frac{ x + 3 } { 2x + 1 }`
encontrar :math: `f * g`

.. math::
	f( x ) = 3x + 2

	g( x ) = \frac{ x + 3 } { 2x + 1 }

	g * f = f[ g(x) ] = 3( \frac { x + 3 } { 2x + 1 } ) + 2

	= ( \frac { 3x + 9 } { 2x + 1 } ) + 2

	= ( \frac { 3x + 9 + 4x + 2 } { 2x + 1 } )
	= ( \frac { 7x + 11 } { 2x + 1 } )

	g * f = f[ g(x) ] = ( \frac { ( 3x + 2 ) + 3 } { 2( 3x + 2 ) + 1 } )
	= ( \frac { 3x + 5 } { 6x + 5 } )

.. math::
	\text{Si} f(a) = b \rightarrow f^-1(b) = a

	f( x ) = 2x

	y = 2x = \frac{ y } { 2 } = x

	y = \frac { x } { 2 }

	f^-1( x ) = \frac{ x } { 2 }

.. math::
	g( x ) = \sqrt[3]{ x - 1 }

	y = \sqrt[3]{ x - 1 }

	y^3 = x - 1

	y^3 + 1 = x

	g^-1( x ) = x^3 + 1
